Adapt definition and proof if cases of theorem

proof/Timing_Function_Analysis.thy
@@ -12,21 +12,22 @@ definition true :: "val \<Rightarrow> bool" where "true v \<equiv> \<not> false 
 
 type_synonym env = "val list"
 
-datatype func = Func string     ("($_)")
+datatype func =
+  Func string     ("($_)")
+| cFunc func    ("(c$_)")
 datatype pfunc = pFunc string   ("(p$_)")
 
 datatype exp =
-    App func "exp list"         ("(_/: _)")
+    App func "exp list"         ("(_/> _)")
   | pApp pfunc "exp list"       ("(_/: _)")
   | If exp exp exp              ("(IF _/ THEN _/ ELSE _)")
   | Ident nat                   ("(i#_)")
   | Const val                   ("(c#_)")
 
-type_synonym t_pApp = "(string \<Rightarrow> val list \<Rightarrow> val)"
-type_synonym defs = "string \<Rightarrow> exp"
+type_synonym defs = "func \<Rightarrow> exp option"
 
 locale timing =
-  fixes pApp :: t_pApp
+  fixes pApp :: "string \<Rightarrow> val list \<Rightarrow> val"
   assumes sum: "pApp ''sum'' es = sum_list es"
 begin
 
@@ -34,17 +35,17 @@ inductive eval :: "env \<Rightarrow> defs \<Rightarrow> exp \<Rightarrow> val \<
 Id:   "\<rho> \<turnstile>\<phi> i#i \<rightarrow> (\<rho> ! i)" |
 C:    "\<rho> \<turnstile>\<phi> c#v \<rightarrow> v" |
 F:    "length es = length vs \<Longrightarrow> (\<forall>i < length vs. \<rho> \<turnstile>\<phi> (es ! i) \<rightarrow> (vs ! i))
-        \<Longrightarrow> \<phi> f = fe \<Longrightarrow> vs \<turnstile>\<phi> fe \<rightarrow> v \<Longrightarrow> \<rho> \<turnstile>\<phi> ($f: es) \<rightarrow> v" |
+        \<Longrightarrow> \<phi> f = Some fe \<Longrightarrow> vs \<turnstile>\<phi> fe \<rightarrow> v \<Longrightarrow> \<rho> \<turnstile>\<phi> (f> es) \<rightarrow> v" |
 P:    "length es = length vs \<Longrightarrow> (\<forall>i < length es. \<rho> \<turnstile>\<phi> (es ! i) \<rightarrow> (vs ! i))
         \<Longrightarrow> pApp p vs = v \<Longrightarrow> \<rho> \<turnstile>\<phi> (p$p: es) \<rightarrow> v" |
-If1:  "\<rho> \<turnstile>\<phi> c \<rightarrow> v \<Longrightarrow> true v \<Longrightarrow> \<rho> \<turnstile>\<phi> t \<rightarrow> v \<Longrightarrow> \<rho> \<turnstile>\<phi> (IF c THEN t ELSE f) \<rightarrow> v" |
-If2:  "\<rho> \<turnstile>\<phi> c \<rightarrow> v \<Longrightarrow> false v \<Longrightarrow> \<rho> \<turnstile>\<phi> f \<rightarrow> v \<Longrightarrow> \<rho> \<turnstile>\<phi> (IF c THEN t ELSE f) \<rightarrow> v"
+If1:  "\<rho> \<turnstile>\<phi> b \<rightarrow> v \<Longrightarrow> true v \<Longrightarrow> \<rho> \<turnstile>\<phi> t \<rightarrow> et \<Longrightarrow> \<rho> \<turnstile>\<phi> (IF b THEN t ELSE f) \<rightarrow> et" |
+If2:  "\<rho> \<turnstile>\<phi> b \<rightarrow> v \<Longrightarrow> false v \<Longrightarrow> \<rho> \<turnstile>\<phi> f \<rightarrow> ef \<Longrightarrow> \<rho> \<turnstile>\<phi> (IF b THEN t ELSE f) \<rightarrow> ef"
 
 inductive_cases IdE[elim!]: "\<rho> \<turnstile>\<phi> i#i \<rightarrow> v"
 inductive_cases CE[elim!]: "\<rho> \<turnstile>\<phi> c#v' \<rightarrow> v"
-inductive_cases FE[elim!]: "\<rho> \<turnstile>\<phi> ($f: es) \<rightarrow> v"
+inductive_cases FE[elim!]: "\<rho> \<turnstile>\<phi> (f> es) \<rightarrow> v"
 inductive_cases PE[elim!]: "\<rho> \<turnstile>\<phi> (p$p: es) \<rightarrow> v"
-inductive_cases IfE[elim!]: "\<rho> \<turnstile>\<phi> (IF c THEN t ELSE f) \<rightarrow> v"
+inductive_cases IfE[elim!]: "\<rho> \<turnstile>\<phi> (IF b THEN t ELSE f) \<rightarrow> v"
 declare Id[simp]
 declare C[simp]
 declare F[simp]
@@ -56,10 +57,16 @@ proposition "\<lbrakk> \<rho> \<turnstile>\<phi> e \<rightarrow> v; \<rho> \<tur
 proof (induction arbitrary: v' rule: eval.induct)
   case (F es vs \<rho> \<phi> f fe v)
   then show ?case
-    by (metis nth_equalityI FE)
+    by (metis FE list_eq_iff_nth_eq option.inject)
 next
   case (P es vs \<rho> \<phi> p v)
   then show ?case by (metis nth_equalityI PE)
+next
+  case (If1 \<rho> \<phi> b v t et f)
+  then show ?case using true_def by blast
+next
+  case (If2 \<rho> \<phi> b v f ef t)
+  then show ?case using true_def by blast
 qed blast+
 
 inductive eval_count :: "env \<Rightarrow> defs \<Rightarrow> exp \<Rightarrow> val * nat \<Rightarrow> bool" ("(_/ \<turnstile>_/ _/ \<rightarrow>s _)") where
@@ -67,17 +74,19 @@ cId:   "\<rho> \<turnstile>\<phi> i#i \<rightarrow>s (\<rho>!i,0)" |
 cC:    "\<rho> \<turnstile>\<phi> c#v \<rightarrow>s (v,0)" |
 cF:    "length es = length vs \<Longrightarrow> length es = length ts
           \<Longrightarrow> (\<And>i. i < length vs \<Longrightarrow> \<rho> \<turnstile>\<phi> (es!i) \<rightarrow>s (vs!i,ts!i))
-          \<Longrightarrow> \<phi> f = fe \<Longrightarrow> vs \<turnstile>\<phi> fe \<rightarrow>s (v,t) \<Longrightarrow> \<rho> \<turnstile>\<phi> ($f: es) \<rightarrow>s (v,1+t+sum_list ts)" |
+          \<Longrightarrow> \<phi> f = Some fe \<Longrightarrow> vs \<turnstile>\<phi> fe \<rightarrow>s (v,t) \<Longrightarrow> \<rho> \<turnstile>\<phi> (f> es) \<rightarrow>s (v,1+t+sum_list ts)" |
 cP:    "length es = length vs \<Longrightarrow> (\<And>i. i < length es \<Longrightarrow> \<rho> \<turnstile>\<phi> (es ! i) \<rightarrow>s (vs!i,ts!i))
           \<Longrightarrow> pApp p vs = v \<Longrightarrow> \<rho> \<turnstile>\<phi> (p$p: es) \<rightarrow>s (v,sum_list ts)" |
-cIf1:  "\<rho> \<turnstile>\<phi> c \<rightarrow>s (v,tc) \<Longrightarrow> true v \<Longrightarrow> \<rho> \<turnstile>\<phi> t \<rightarrow>s (v,tt) \<Longrightarrow> \<rho> \<turnstile>\<phi> (IF c THEN t ELSE f) \<rightarrow>s (v,tc+tt)" |
-cIf2:  "\<rho> \<turnstile>\<phi> c \<rightarrow>s (v,tc) \<Longrightarrow> false v \<Longrightarrow> \<rho> \<turnstile>\<phi> f \<rightarrow>s (v,tf) \<Longrightarrow> \<rho> \<turnstile>\<phi> (IF c THEN t ELSE f) \<rightarrow>s (v,tc+tf)"
+cIf1:  "\<rho> \<turnstile>\<phi> b \<rightarrow>s (eb,tb) \<Longrightarrow> true eb \<Longrightarrow> \<rho> \<turnstile>\<phi> t \<rightarrow>s (et,tt)
+          \<Longrightarrow> \<rho> \<turnstile>\<phi> (IF b THEN t ELSE f) \<rightarrow>s (et,tb+tt)" |
+cIf2:  "\<rho> \<turnstile>\<phi> b \<rightarrow>s (eb,tb) \<Longrightarrow> false eb \<Longrightarrow> \<rho> \<turnstile>\<phi> f \<rightarrow>s (ef,tf)
+          \<Longrightarrow> \<rho> \<turnstile>\<phi> (IF b THEN t ELSE f) \<rightarrow>s (ef,tb+tf)"
 
 inductive_cases cIdE[elim!]: "\<rho> \<turnstile>\<phi> i#i \<rightarrow>s v"
 inductive_cases cCE[elim!]: "\<rho> \<turnstile>\<phi> c#v' \<rightarrow>s v"
-inductive_cases cFE[elim!]: "\<rho> \<turnstile>\<phi> ($f: es) \<rightarrow>s v"
+inductive_cases cFE[elim!]: "\<rho> \<turnstile>\<phi> (f> es) \<rightarrow>s v"
 inductive_cases cPE[elim!]: "\<rho> \<turnstile>\<phi> (p$p: es) \<rightarrow>s v"
-inductive_cases cIfE[elim!]: "\<rho> \<turnstile>\<phi> (IF c THEN t ELSE f) \<rightarrow>s v"
+inductive_cases cIfE[elim!]: "\<rho> \<turnstile>\<phi> (IF b THEN t ELSE f) \<rightarrow>s v"
 declare cId[intro]
 declare cC[intro]
 declare cF[intro]
@@ -85,11 +94,7 @@ declare cP[intro]
 declare cIf1[intro]
 declare cIf2[intro]
 
-thm exI[of _ "[undefined]"]
-lemma Ex_list_of_length: "\<exists>xs. length xs = n"
-by (rule exI[of _ "replicate n undefined"]) simp
-
-lemma helper:
+lemma eval_eval_count':
   assumes "\<And>i. i < length vs \<Longrightarrow> \<exists>t. \<rho> \<turnstile>\<phi> es ! i \<rightarrow>s (vs ! i, t)"
   and "length vs = length es"
   shows  "\<exists>ts. length vs = length ts \<and> (\<forall>i. (i < length vs \<longrightarrow> \<rho> \<turnstile>\<phi> (es!i) \<rightarrow>s (vs!i,ts!i)))"
@@ -114,68 +119,114 @@ proof (induction vs arbitrary: es)
     using ts t e
     by (metis Suc_less_eq length_Cons not0_implies_Suc nth_Cons_0 nth_Cons_Suc)
 
-  ultimately
-  show ?case by blast
+  ultimately show ?case by blast
 qed simp
 
-lemma eval_eval_count: "(\<rho> \<turnstile>\<phi> c \<rightarrow> v \<Longrightarrow> \<exists>t. \<rho> \<turnstile>\<phi> c \<rightarrow>s (v,t))"
+lemma eval_eval_count: "\<rho> \<turnstile>\<phi> b \<rightarrow> v \<Longrightarrow> \<exists>t. \<rho> \<turnstile>\<phi> b \<rightarrow>s (v,t)"
 proof (induction rule: eval.induct)
   case (F es vs \<rho> \<phi> f fe v)
   then show ?case
-    by (metis cF helper)
+    by (metis cF eval_eval_count')
 next
   case (P es vs \<rho> \<phi> p v)
   then show ?case
-    by (metis cP helper)
+    by (metis cP eval_eval_count')
 qed blast+
 
-lemma eval_count_eval: "\<rho> \<turnstile>\<phi> c \<rightarrow>s (v,t) \<Longrightarrow> \<rho> \<turnstile>\<phi> c \<rightarrow> v"
-  by (induction \<rho> \<phi> c "(v,t)" arbitrary: v t rule: eval_count.induct) auto
+lemma eval_count_eval: "\<rho> \<turnstile>\<phi> b \<rightarrow>s (v,t) \<Longrightarrow> \<rho> \<turnstile>\<phi> b \<rightarrow> v"
+  by (induction \<rho> \<phi> b "(v,t)" arbitrary: v t rule: eval_count.induct) auto
 
-lemma  eval_eq_eval_count: "(\<rho> \<turnstile>\<phi> c \<rightarrow> v) \<longleftrightarrow> (\<exists>t. \<rho> \<turnstile>\<phi> c \<rightarrow>s (v,t))"
+theorem  eval_eq_eval_count: "(\<rho> \<turnstile>\<phi> b \<rightarrow> v) \<longleftrightarrow> (\<exists>t. \<rho> \<turnstile>\<phi> b \<rightarrow>s (v,t))"
   using eval_count_eval eval_eval_count by auto
 
 (* TODO: define T and proove:
 proposition "\<rho> \<turnstile>\<phi> e \<rightarrow>s (v,t) \<longleftrightarrow> \<rho> \<turnstile>\<phi> e \<rightarrow> v \<and> T \<Delta> = t"
-
 *)
 
 fun \<T> :: "exp \<Rightarrow> exp" where
   "\<T> c#v = c#0"
 | "\<T> i#i = c#0"
-| "\<T> (IF c THEN t ELSE f) = p$''sum'': [\<T> c, IF c THEN \<T> t ELSE \<T> f]"
+| "\<T> (IF b THEN t ELSE f) = p$''sum'': [\<T> b, IF b THEN \<T> t ELSE \<T> f]"
 | "\<T> (p$_: args) = p$''sum'': map \<T> args"
-| "\<T> ($f: args) = p$''sum'': ($f:args # map \<T> args)"
-                  
-definition c :: "defs \<Rightarrow> defs" where
-  "c \<phi> f = p$''sum'': [c#1, \<T> (\<phi> f)]"
+| "\<T> (f> args) = p$''sum'': (c$f> args # map \<T> args)"
 
-text \<open>Small example\<close>
-lemma add2: "\<rho> \<turnstile>\<phi> (p$''sum'': [c#n, c#m]) \<rightarrow> n+m"
-proof -
-  have 1: "\<rho> \<turnstile>\<phi> c#n \<rightarrow> n" by simp
-  have 2: "\<rho> \<turnstile>\<phi> c#m \<rightarrow> m" by simp
+fun c :: "exp \<Rightarrow> exp" where
+  "c e = p$''sum'': [c#1, \<T> e]"
 
-  have len: "length [c#n,c#m] = length [n,m]" by simp
-  from 1 2 have li: "\<forall>i < length [n,m]. \<rho> \<turnstile>\<phi> ([c#n,c#m] ! i) \<rightarrow> ([n,m] ! i)"
-    by (simp add: nth_Cons')
-  have pApp: "pApp ''sum'' [n,m] = n+m" by (auto simp: sum)
+fun conv :: "defs \<Rightarrow> defs" where
+  "conv \<phi> (c$f) = (case \<phi> f of None \<Rightarrow> None | Some e \<Rightarrow> Some (c e))"
+| "conv \<phi> ($f) = \<phi> $f"
 
-  from len li pApp P[of "[c#n,c#m]" "[n,m]" \<rho> \<phi> "''sum''" "n+m"]
-  show ?thesis by simp
-qed
+definition defs_cor where
+  "defs_cor \<phi> =
+  (\<forall>f. (case \<phi> f of Some e \<Rightarrow> \<phi> (c$f) = None \<or> \<phi> (c$f) = Some (c e)
+                  | None \<Rightarrow> \<phi> (c$f) = None))"
 
-fun \<phi> :: "defs" where
-  "\<phi> s = c#0"
+lemma conv_trans: "defs_cor \<phi> \<Longrightarrow> \<phi> f = Some e \<Longrightarrow> (conv \<phi>) f = Some e"
+  apply (cases f)
+  by auto (smt (verit, best) conv.simps(1) defs_cor_def option.case_eq_if option.distinct(1))
 
-lemma "\<rho> \<turnstile>\<phi> ($''callee'': []) \<rightarrow> 0"
-  by (rule F) auto
+lemma eval_conv_trans: "\<rho> \<turnstile>\<phi> e \<rightarrow> v \<Longrightarrow> defs_cor \<phi> \<Longrightarrow> \<rho> \<turnstile>(conv \<phi>) e \<rightarrow> v"
+  by (induction rule: eval.induct) (auto simp: conv_trans)
 
-lemma "\<rho> \<turnstile>(c \<phi>) ($''callee'': []) \<rightarrow> 1"
-  apply (rule F)
-  apply (auto simp: c_def)
-  using add2[of "[]" "c \<phi>" 1 0]
-  by simp
+theorem
+  assumes "\<rho> \<turnstile>\<phi> e \<rightarrow>s (s,t)"
+    and   "defs_cor \<phi>"
+  shows  "\<rho> \<turnstile>(conv \<phi>) (\<T> e) \<rightarrow> t"
+  using assms
+proof (induction \<rho> \<phi> e "(s,t)" arbitrary: s t rule: eval_count.induct)
+  case (cF es vs ts \<rho> \<phi> f fe v t)
+  then show ?case sorry
+next
+  case (cP es vs \<rho> \<phi> ts p v)
+  then show ?case sorry
+next
+  case (cIf1 \<rho> \<phi> b eb tb t et tt f)
+
+  let ?ts = "[\<T> b, IF b THEN \<T> t ELSE \<T> f]"
+
+  have "\<rho> \<turnstile>\<phi> b \<rightarrow> eb"
+    using cIf1(1) eval_count_eval by auto
+
+  then have b: "\<rho> \<turnstile>(conv \<phi>) b \<rightarrow> eb"
+    using cIf1.prems eval_conv_trans by auto
+
+  from b cIf1(3) cIf1(5)
+  have ifelse: "\<rho> \<turnstile>(conv \<phi>) IF b THEN \<T> t ELSE \<T> f \<rightarrow> tt"
+    by (simp add: cIf1.prems)
+
+  from cIf1(2) ifelse
+  have args: "(\<forall>i < length ?ts. \<rho> \<turnstile>(conv \<phi>) (?ts ! i) \<rightarrow> ([tb,tt] ! i))"
+    by (simp add: cIf1.prems nth_Cons')
+  have app: "pApp ''sum'' [tb,tt] = tb + tt" by (simp add: timing.sum timing_axioms)
+
+  from args app P[of ?ts "[tb,tt]"]
+  have "\<rho> \<turnstile>conv \<phi> (p$''sum'': ?ts) \<rightarrow> tb + tt" by simp
+  then show ?case by simp
+next
+  case (cIf2 \<rho> \<phi> b eb tb f ef tf t)
+
+  let ?ts = "[\<T> b, IF b THEN \<T> t ELSE \<T> f]"
+
+  have "\<rho> \<turnstile>\<phi> b \<rightarrow> eb"
+    using cIf2(1) eval_count_eval by auto
+
+  then have b: "\<rho> \<turnstile>(conv \<phi>) b \<rightarrow> eb"
+    using cIf2.prems eval_conv_trans by auto
+
+  from b cIf2(3) cIf2(5)
+  have ifelse: "\<rho> \<turnstile>(conv \<phi>) IF b THEN \<T> t ELSE \<T> f \<rightarrow> tf"
+    by (simp add: cIf2.prems)
+
+  from cIf2(2) ifelse
+  have args: "(\<forall>i < length ?ts. \<rho> \<turnstile>(conv \<phi>) (?ts ! i) \<rightarrow> ([tb,tf] ! i))"
+    by (simp add: cIf2.prems nth_Cons')
+  have app: "pApp ''sum'' [tb,tf] = tb + tf" by (simp add: timing.sum timing_axioms)
+
+  from args app P[of ?ts "[tb,tf]"]
+  have "\<rho> \<turnstile>conv \<phi> (p$''sum'': ?ts) \<rightarrow> tb + tf" by simp
+  then show ?case by simp
+qed simp+
 
 end
 
